src/tls/StreamAE.fst
@@ -16,6 +16,8 @@ open TLSError
 open TLSConstants
 open TLSInfo
 open StreamPlain
+open MonotoneSeq
+open FStar.Monotonic.RRef
 
 type id = i:id { pv_of_id i = TLS_1p3 }
 
@@ -44,12 +46,14 @@ let max_uint64 =
   let n = 1073741823 in //2^30-1 4611686018427387903 in // (2^62-1) (* TODO: Fix this *)
   lemma_repr_bytes_values n; n
 
+type log_ref (r:rid) (i:id)  = FStar.Monotonic.RRef.m_rref r (seq (entry i)) MonotoneSeq.grows
+
 type state (i:id) (rw:rw) =
   | State: #region:rid 
          -> #peer_region:rid{HyperHeap.disjoint region peer_region}
          -> key:key i
          -> iv: iv i
-         -> log: rref (if rw=Reader then peer_region else region) (seq (entry i)) // ghost, subject to cryptographic assumption
+         -> log: log_ref (if rw=Reader then peer_region else region) i // ghost, subject to cryptographic assumption
          -> counter: rref region (seqn i) // types are sufficient to anti-alias log and counter
          -> state i rw
 // Some invariants:
@@ -77,13 +81,13 @@ val gen: reader_parent:rid -> writer_parent:rid -> i:id -> ST (reader i * writer
          /\ extends (r.region) reader_parent
          /\ fresh_region w.region h0 h1
          /\ fresh_region r.region h0 h1
-         /\ op_Equality #(rref w.region (seq (entry i))) w.log r.log  //the explicit annotation here *)
+         /\ op_Equality #(log_ref w.region i) w.log r.log  //the explicit annotation here *)
          /\ contains_ref w.counter h1
          /\ contains_ref r.counter h1
-         /\ contains_ref w.log h1
+         /\ m_contains w.log h1
          /\ 0 = sel h1 w.counter
          /\ 0 = sel h1 r.counter
-         /\ sel h1 w.log = createEmpty
+         /\ m_sel h1 w.log = createEmpty
          ))
 
 let gen reader_parent writer_parent i =
@@ -94,7 +98,7 @@ let gen reader_parent writer_parent i =
   lemma_repr_bytes_values 0;
   let ectr = ralloc writer_r 0 in
   let dctr = ralloc reader_r 0 in
-  let log  = ralloc writer_r Seq.createEmpty in
+  let log  = alloc_mref_seq writer_r Seq.createEmpty in 
   let writer  = State #i #Writer #writer_r #reader_r kv iv log ectr in
   let reader  = State #i #Reader #reader_r #writer_r kv iv log dctr in
   reader, writer
@@ -114,15 +118,15 @@ let coerce r0 p0 i role kv iv =
   lemma_repr_bytes_values 0;
   let ctr : rref r _ = ralloc r 0 in
   if role=Reader
-  then let log : rref p _ = ralloc p Seq.createEmpty in
+  then let log = alloc_mref_seq p Seq.createEmpty in 
        State #i #role #r #p kv iv log ctr
-  else let log : rref r _ = ralloc r Seq.createEmpty in
-       State #i #role #r #p kv iv log ctr //NS: worryingly, succeeds with implicit arguments even without the role=Writer
+  else let log = alloc_mref_seq r Seq.createEmpty in
+       State #i #role #r #p kv iv log ctr 
+
 
 val leak: i:id{~(safeId i)} -> role:rw -> state i role -> ST (key i * iv i)
   (requires (fun h0 -> True))
   (ensures  (fun h0 r h1 -> modifies Set.empty h0 h1 ))
-
 let leak i role s = State.key s, State.iv s
 
 
@@ -142,7 +146,7 @@ let aeIV i (n:seqn i) (staticIV: iv i) : iv i =
 
 // not relying on additional data
 let noAD = empty_bytes
-
+ 
 // Raw encryption (on concrete bytes), returns (cipher @| tag)
 // Keeps seqn and nonce implicit; requires the counter not to overflow
 val enc:
@@ -151,6 +155,7 @@ val enc:
     (ensures  (fun h0 c h1 ->
                  modifies (Set.singleton e.region) h0 h1
                /\ modifies_rref e.region !{as_ref e.counter} h0 h1
+	       /\ contains_ref e.counter h1
                // /\ sel h1 e.counter = sel h0 e.counter + 1
     ))
 
@@ -172,6 +177,9 @@ let enc i e l p =
     end;
    c
 
+(* val encrypted : #r:rid -> #i:id -> log:log_ref r i -> e:entry i -> h:HyperHeap.t -> GTot Type0 *)
+(* let encrypted #r #i log e = MonotoneSeq.mem e log *)
+
 
 // encryption of plaintexts; safe instances are idealized
 val encrypt:
@@ -179,23 +187,25 @@ val encrypt:
     (requires (fun h0 -> True))
     (ensures  (fun h0 c h1 ->
                            modifies (Set.singleton e.region) h0 h1
-                         /\ modifies_rref e.region !{as_ref e.counter, as_ref e.log} h0 h1
-                         /\ contains_ref e.log h1
+                         /\ modifies_rref e.region !{as_ref e.counter, as_ref (as_rref e.log)} h0 h1
+                         /\ m_contains e.log h1
                          /\ contains_ref e.counter h1
                          (* /\ sel h1 e.counter = sel h0 e.counter + 1 *)
-                         /\ sel h1 e.log = snoc (sel h0 e.log) (Entry l c p)))
+			 /\ (let ent = Entry l c p in
+   			      witnessed (MonotoneSeq.mem ent e.log)
+                           /\  m_sel h1 e.log = snoc (m_sel h0 e.log) ent)))
 
 (* we primarily model the ideal functionality, the concrete code that actually
    runs on the network is what remains after dead code elimination when
    safeId i is fixed to false and after removal of the cryptographic ghost log,
    i.e. all idealization is turned off *)
-#reset-options
 let encrypt i e l p =
-  recall e.log;   recall e.counter;
+  m_recall e.log;  
+  recall e.counter;
   let text = if safeId i then createBytes l 0uy else repr i l p in
   let c = enc i e l text in
-  e.log := snoc !e.log (Entry l c p);
-  recall e.counter;
+  let ent = Entry l c p in
+  MonotoneSeq.write_at_end e.log ent;
   c
 
 
@@ -223,7 +233,7 @@ val decrypt:
   (ensures  (fun h0 res h1 ->
                modifies Set.empty h0 h1
              /\ (authId i ==>
-                 (let log :seq (entry i) = sel h0 d.log in
+                 (let log :seq (entry i) = m_sel h0 d.log in
 		   match res with
 		     | None -> forall (j:nat{j < Seq.length log}).{:pattern (found j)}
                                             found j /\ ~(matches l c (Seq.index log j))
@@ -235,8 +245,8 @@ val decrypt:
 
 // decryption, idealized as a lookup of (c,ad) in the log for safe instances
 let decrypt i d l c =
-  recall d.log;
-  let log = !d.log in
+  m_recall d.log;
+  let log = m_read d.log in
   if authId i then
     match seq_find (matches l c) log with
     | None -> None
